theories/Simple/SimplePipeline.v
@@ -1,13 +1,17 @@
 From Coq Require Import Program.
 From MetaCoq.Utils Require Import utils.
-From MetaCoq.Common Require Import Transform config.
+From MetaCoq.Common Require Import BasicAst Transform config.
+From MetaCoq.Template Require Import TemplateMonad Loader.
+From MetaCoq.Erasure Require Import EAst EProgram EWcbvEval.
+From MetaCoq.ErasurePlugin Require Import Erasure Loader.
 
-From VTL.Simple Require Import DBToPIR.
+From VTL.Simple Require Import EAstToDB DBToPIR.
 From VTL.Semantics Require Import BigStepPIR.
 
 (* A end-to-end pipeline from Coq/Gallina terms to PIR terms (with bogus types):
    Gallina ▷ TemplateRocq ▷ PCUIC ▷ λ□/EAst (without box type annotations) ▷ DB ▷ PIR *)
 
+Import MCMonadNotation.
 Import Common.Transform.Transform.
 #[local] Obligation Tactic := program_simpl.
 
@@ -17,32 +21,119 @@ Definition tm_program  := unit × tm.
 Definition pir_program := unit × term.
 
 Definition eval_tm_program  (p : tm_program)  (v  : tm)   := ∥ DBToPIR.eval p.2 v ∥.
-Definition eval_pir_program (p : pir_program) (v' : term) := ∥ BigStepPIR.eval p.2 v' default_pir_fuel ∥.
+Definition eval_pir_program (p : pir_program) (v' : term) := ∥ exists k, BigStepPIR.eval p.2 v' k ∥.
 
-Axiom translate_named : tm -> term.
-Definition translate_named_program (p : tm_program) := (tt, translate_named p.2).
+Definition translatable_et (p : eprogram) : Prop :=
+  let '(_, et) := p in
+  exists t, translate_et [] et = Some t.
+Definition translate_erased_program p (pre : translatable_et p) := 
+  match translate_et [] p.2 with
+  | Some t => (tt, t)
+  | None => (tt, tm_oops) end.
+
+Definition translatable_tm (p : tm_program) : Prop := 
+  let '(_, t) := p in
+  exists t', translate_term [] t = Some t'. 
+Definition translate_stlc_program p (pre : translatable_tm p) := (tt, translate_unsafe p.2).
+
+Program Definition east_to_stlc_transform :
+  Transform.t global_context unit EAst.term tm EAst.term tm
+  (eval_eprogram final_wcbv_flags) 
+  eval_tm_program :=
+  {| name := "translate lambda box to stlc" ;
+     pre := translatable_et ;
+     transform := translate_erased_program ;
+     post _ := True ;
+     obseq ep _ p ev v := True ;
+     preservation _ _ _ _ := _
+  |}.
+Next Obligation.
+  unfold translatable_et in t1.
+  destruct p as [env et] eqn:H.
+  destruct t1 as [t2 tl].
+  destruct e. exists t2.
+  split. unfold eval_tm_program. sq.
+  unfold translate_erased_program. simpl. 
+  rewrite tl. simpl in *.
+Admitted.
+
+(* Lemma translate_program_correct *)
+
+Lemma compose_translate_term : forall Γ t t',
+  translate_et Γ t = Some t' ->
+  exists t'', translate_term (map bytestring.String.to_string Γ) t' = Some t''.
+Proof.
+Admitted.
+
+Lemma compose_translatable : forall p,
+  translatable_et p ->
+  exists p', translatable_tm p'.
+Proof.
+  intros p tl.
+  destruct p.
+  unfold translatable_et in tl.
+  destruct tl. apply compose_translate_term in H as [t'' H'].
+  exists (tt, x). unfold translatable_tm. exists t''. simpl in H'.
+  assumption.
+Admitted.
 
 Program Definition stlc_to_pir_transform :
   Transform.t unit unit tm term tm term
   eval_tm_program
   eval_pir_program :=
   {| name := "translate stlc to pir terms";
-     transform input _ := _;
-     obseq p _ p' v v' := translatesTo [] v v' ;
+     pre := translatable_tm;
+     transform := translate_stlc_program;
+     post _ := True;
+     obseq p _ p' v v' := translatesTo [] v v';
+     preservation _ _ _ _ := _
   |}.
 Next Obligation.
-(* pre? *) exact True.
+  unfold translatable_tm in t1.
+  destruct p as [env t] eqn:H.
+  destruct t1 as [t' tl].
+  destruct e.
+  specialize (translate_correct t t0 t' H0 tl).
+  unfold translate_stlc_program. unfold eval_pir_program.
+  intros tlt.
+  destruct tlt as [v' [fuel [tlt ev]]].
+  exists v'. split.
+  - sq. exists fuel. simpl. 
+    unfold translate_unsafe. 
+    now rewrite tl.
+  - assumption.
 Qed.
+
+Program Definition partial_pipeline :
+  Transform.t _ _ _ term _ term
+  (eval_eprogram final_wcbv_flags) 
+  eval_pir_program :=
+  east_to_stlc_transform ▷
+  stlc_to_pir_transform.
 Next Obligation.
-(* pre is true of input *) Admitted.
-Next Obligation.
-(* post *) exact True.
-Qed.
-Next Obligation.
-(* pre establishes post *)
-Admitted.
-Next Obligation.
-  (* exact (translate_correct p.2 v p'.2 (∥ evalNamed p.2 v ∥) (∥ eval p'.2 v'∥)). *)
 Admitted.
 
-Check run stlc_to_pir_transform.
+Program Definition simple_pipeline :
+  Transform.t _ _ _ term _ term
+  _ 
+  eval_pir_program :=
+  erasure_pipeline_mapping ▷
+  east_to_stlc_transform ▷
+  stlc_to_pir_transform.
+Next Obligation.
+(* well-formed implies translatable, needs subset condition *)
+Admitted.
+Next Obligation.
+(* tl et = Some t -> tl t = Some et *)
+Admitted.
+
+Import Strings.String.
+
+Axiom assume_translatable : forall p, pre simple_pipeline ([], p).
+
+Definition compile_pir (p : Ast.Env.program) : PIR.term :=
+  (run simple_pipeline ([], p) (assume_translatable p)).2.
+
+Eval vm_compute in <# (fun (x : bool) => x) true #>.
+Eval vm_compute in (run erasure_pipeline_mapping ([], <# (fun (x : bool) => x) true #>)) _.
+Eval vm_compute in compile_pir <# (fun (x : bool) => x) true #>.
