theories/Simple/EAstToDB.v
@@ -1,0 +1,34 @@
+From MetaCoq.Erasure Require Import EAst.
+From MetaCoq.Utils Require Import utils.
+Import BasicAst Kernames MCMonadNotation.
+
+From VTL Require Import DBToPIR.
+
+From Coq Require Import String BinInt List.
+Import ListNotations.
+
+Local Open Scope string_scope.
+
+Notation "'bs_to_s' s" := (bytestring.String.to_string s) (at level 200).
+Notation "'s_to_bs' s" := (bytestring.String.of_string s) (at level 200).
+Local Coercion bytestring.String.to_string : bytestring.String.t >-> string.
+
+(* hallucinates simple types for tm, maybe add synth_type *)
+Fixpoint translate_et (Γ : list bs) t : option tm :=
+  match t with
+  | tConstruct _ _ _ => Some tm_true
+  | tRel k => match nth_error Γ k with
+              | Some _ => Some (tm_rel k)
+              | None => None end
+  | tLambda (nNamed x) b => 
+      b' <- translate_et (x :: Γ) b ;;
+      Some (tm_abs x (Ty_Arrow Ty_Bool Ty_Bool) b')
+  | tApp s t =>
+      s' <- translate_et Γ s ;;
+      t' <- translate_et Γ t ;;
+      Some (tm_app s' t')
+  | _ => None
+  end.
+
+Definition tru := (tLambda (nNamed "t"%bs) (tLambda (nNamed "f"%bs) (tRel 0))).
+Eval cbv in translate_et [] tru.
